\documentclass{article}

\usepackage{amsmath}
\usepackage{amssymb}
\usepackage[
  left=1cm,
  right=1cm,
  top=2cm,
  bottom=2cm,
]{geometry}

\begin{document}

\section*{Klausur}
\subsection*{A}
a)\\
\begin{align*}
    \frac{(2+i)^2}{1-i} = \frac{3+4i}{1-i} = \frac{(3+4i)(1+i)}{(1-i)(1+i)} = -\frac{1+7i}{2}
\end{align*}
\begin{align*}
    \lvert z \rvert &= 2 = r^2 \text{und} \mathrm{arg} (z) = \pi\\
    2e^{i\pi} &= 2 \left(\cos \pi + i \sin \pi\right)\\
    &= -2
\end{align*}
b)
\begin{center}
    \begin{tabular}{c c c c c c c}
        \hline
        n & 0 & 1 & 2 & 3 & 4 & 5\\
        \hline
        $a_n$ & $-\frac{-1}{1}$ & $\frac{0}{3}$ & $-\frac{1}{5}$ & $\frac{2}{7}$ & $-\frac{3}{9}$ & $\frac{4}{11}$\\
    \end{tabular}
\end{center}
\begin{align*}
    a_n &= \frac{n-1}{2n+1}\cdot (-1)^{n+1}
\end{align*}
c)
\begin{align*}
    P_1(-1,4),\,P_2(1,4),\,P_3(2,13)\\
    P_2(x) &= c_0 + c_1 (x-x_0) + c_2 (x_1-x_1)(x_1 - x_0)\\
    P_2(x_0) &= P_2(-1) = c_0 = 4\\
    P_2(x_1) &= P_2(1) = 4+c_1(x_1-x_0)+c_2(x_1-x_1)(x_1-x_0)\\
    &= 4+c_1(1-(-1))\\
    4 &= 4+2c_1\\
    c_1 &= 0\\\\
    P_2(2) &= 4 + c_2(2-1)(2-(-1))\\
    13 &= 4+ c_2 \cdot 1 \cdot 3\\
    9 &= 3c_2\\
    c_2 &= 3\\\\
    \Rightarrow P_2(x) &= 4+0(x+1)+3(x-1)(x+1)\\
    &= 4+3(x^2-x+x-1)\\
    &= 4+3x^2-3\\
    &= 3x^2+1
\end{align*}

d)
\begin{align*}
    f(x) &= 3x^2+1 [-\pi ,\,\pi ]\\
    c_0 &= \frac{1}{\sqrt{2\pi}} \int_{-\pi}^{\pi} \left(3x^2+1\right)r^{-i\cdot 0 \cdot x}\,dx\\
    &= \frac{1}{\sqrt{2\pi}} \left[x^3+x\right]_{-\pi}^{\pi}\\
    &= \frac{1}{\sqrt{2\pi}} \left[\pi^3+\pi-\left(-\pi^3-\pi\right)\right]\\
    &= \frac{1}{\sqrt{2\pi}}\left(2\pi^3+2\pi\right)\\
    &= \sqrt{2\pi} \left(\pi^2+1\right)\\\\
    c_k &= \frac{1}{\sqrt{2\pi}} \int_{-\pi}^{\pi} \left(3x^2+1\right)3^{-ikx}\,dx\\
    &= \frac{1}{\sqrt{2\pi}} \int_{-\pi}^{\pi}e^{-ikx}\,dx + \frac{1}{\sqrt{2\pi}} \int_{-\pi}^{\pi} 3x^2e^{-ikx}\,dx\\
    f(x) =3x^2,\,f'(x) = 6x\\
    g'(x) =e^{-ikx},\,g(x) =\frac{e^-ikx}{-ik}\\
    &= \frac{1}{\sqrt{2\pi}}\left[\frac{e^{-ikx}}{-ik}\right]_{-\pi}^{\pi} + \frac{1}{\sqrt{2\pi}}\left[3x^2\frac{e^{-ikx}}{-ik}\right]_{-\pi}^{\pi} - \frac{1}{\sqrt{2\pi}}\int_{-\pi}^{\pi} 6x \frac{e^{-ikx}}{-ik}\,dx\\
    &= 0 + 0 - \frac{1}{\sqrt{2\pi}}\int_{-\pi}^{\pi} 6x \frac{3^{-ikx}}{-ik}\,dx\\
    c_k &= - \frac{1}{\sqrt{2\pi}}\int_{-\pi}^{\pi} 6x \frac{e^{-ikx}}{-ik}\,dx\\
    f(x) =3x^2,\,f'(x) = 6x\\
    g'(x) =e^{-ikx},\,g(x) =\frac{e^-ikx}{-ik}\\
    &= \frac{1}{\sqrt{2\pi}ik} \left[6x\frac{3^{-ikx}}{-ik}\right]_{-\pi}^{\pi}-\frac{1}{\sqrt{2\pi}ik}\int_{-\pi}^{\pi} 6\frac{e^{-ikx}}{-ik}\,dx\\
    &= \frac{1}{\sqrt{2\pi}(-i)ik^2} \left[6xe^{-ikx}\right]_{-\pi}^{\pi}-\frac{1}{\sqrt{2\pi}(-i)ik^2}\left[6\frac{e^{-ikx}}{-ik}\right]_{-\pi}^{\pi}\\
    &= \frac{6}{\sqrt{2\pi}k^2}\left[xe^{-ikx}\right]_{-\pi}^{\pi}-\frac{6}{\sqrt{2\pi}k^2}\left[\frac{e^{-ikx}}{-ik}\right]_{-\pi}^{\pi}\\
    c_k &= \frac{6}{\sqrt{2\pi}k^2}(2\pi)e^{-ikx}\\
    &= \frac{6\sqrt{2\pi}}{k^2}(-1)^k
\end{align*}
\begin{align*}
    f(x)&=\frac{1}{\sqrt{2\pi}}\sqrt{2\pi}(\pi^2+1)+\frac{1}{\sqrt{2\pi}}\sum_{-\infty}^{\infty} \frac{6\sqrt{2\pi} (-1)^k}{k^2}e^{ikx}\\
    &= \pi^2 + 1+\sum_{-\infty}^{\infty} \frac{6(-1)^k}{k^2}e^{ikx}
\end{align*}

\subsubsection*{B}
\begin{align*}
    A_k &= \left(\begin{matrix}
        k & -1 & -3\\
        0 & -k & 2\\
        k & 0 & k
    \end{matrix}\right)\\
    &= \det (A_k)\\
    &= -k(k+1)(k+2)\\\\
    \det(A) &\neq 0\\
    k &= 0,\, -1,\, -2\\\\
    A_1 &= \left(\begin{matrix}
        1&-1&-3\\0&-1&3\\1&0&1
    \end{matrix}\right)\\
    &= A_1 A_1^{-1} = E\\
\end{align*}
\end{document}